Use Timestamp instead of PerfReport and Timetamped instead of Tagged

ironfleet/src/Dafny/Distributed/Common/Framework/Timestamp.s.dfy
@@ -3,17 +3,17 @@ include "Host.s.dfy"
 include "DistributedSystem.s.dfy"
 include "../Collections/Seqs.i.dfy"
 
-abstract module Performance_s {
+abstract module Timestamp_s {
   import opened Collections__Seqs_i
   import opened DS_s : DistributedSystem_s
 
-  type PerfObject = i : int | 0 <= i
+  type Timestamp = i : int | 0 <= i
 
-  function {:axiom} PerfMax(p1:PerfObject, p2:PerfObject) : PerfObject
-    // ensures PerfMax(p1, p2) >= p1 && PerfMax(p1, p2) >= p2
-    // ensures PerfMax(p1, p2) == p1 || PerfMax(p1, p2) == p2
-    ensures p1 >= p2 ==> PerfMax(p1, p2) == p1
-    ensures p2 >= p1 ==> PerfMax(p1, p2) == p2
+  function {:axiom} TimeMax(p1:Timestamp, p2:Timestamp) : Timestamp
+    // ensures TimeMax(p1, p2) >= p1 && TimeMax(p1, p2) >= p2
+    // ensures TimeMax(p1, p2) == p1 || TimeMax(p1, p2) == p2
+    ensures p1 >= p2 ==> TimeMax(p1, p2) == p1
+    ensures p2 >= p1 ==> TimeMax(p1, p2) == p2
   {
     if p1 < p2 then
       p2
@@ -21,28 +21,26 @@ abstract module Performance_s {
       p1
   }
 
-  function PerfZero() : PerfObject
+  function TimeZero() : Timestamp
   {
     0
   }
 
-  function PerfVoid() : PerfObject
+  function TimeVoid() : Timestamp
   {
     0
   }
 
-  function {:axiom} PerfDelivery() : imap<nat, PerfObject>
-    ensures imaptotal(PerfDelivery())
+  function {:axiom} DeliveryTime() : imap<nat, Timestamp>
+    ensures imaptotal(DeliveryTime())
 
-  function {:axiom} PerfStep(hstep:HostStep) : imap<nat, PerfObject>
-    ensures imaptotal(PerfStep(hstep))
+  function {:axiom} StepTime(hstep:HostStep) : imap<nat, Timestamp>
+    ensures imaptotal(StepTime(hstep))
 
-  function PerfAdd2(p1:PerfObject, p2:PerfObject) : PerfObject
+  function TimeAdd2(p1:Timestamp, p2:Timestamp) : Timestamp
   {
     p1 + p2
   }
-
-  type PerfExpr = PerfObject
 
   datatype NumSteps = NumSteps(num_hsteps:imap<HostStep, nat>, num_deliveries:nat)
     
@@ -57,25 +55,25 @@ abstract module Performance_s {
     NumSteps(imap h:HostStep | true :: 0 as nat , 0)
   }
 
-  function NoRecvPerfUpdate(node_pr:PerfExpr, hstep:HostStep, num_steps:NumSteps) : (PerfExpr, NumSteps)
+  function NoRecvTimestampUpdate(node_ts:Timestamp, hstep:HostStep, num_steps:NumSteps) : (Timestamp, NumSteps)
     requires ValidNumSteps(num_steps)
     ensures ValidNumSteps(num_steps)
   {
     var step_idx := num_steps.num_hsteps[hstep];
-    var total_time := PerfAdd2(node_pr, PerfStep(hstep)[step_idx]);
+    var total_time := TimeAdd2(node_ts, StepTime(hstep)[step_idx]);
     var num_steps' := num_steps.(num_hsteps := num_steps.num_hsteps[hstep := num_steps.num_hsteps[hstep] + 1]);
     (total_time, num_steps')
   }
 
-  function RecvPerfUpdate(node_pr:PerfExpr, pkt_pr:PerfExpr, hstep:HostStep, num_steps:NumSteps) : (PerfExpr, NumSteps)
+  function RecvTimestampUpdate(node_ts:Timestamp, pkt_ts:Timestamp, hstep:HostStep, num_steps:NumSteps) : (Timestamp, NumSteps)
     requires ValidNumSteps(num_steps)
     ensures ValidNumSteps(num_steps)
   {
     var delivery_idx := num_steps.num_deliveries;
-    var deliveryTime := PerfAdd2(pkt_pr, PerfDelivery()[delivery_idx]);
-    var handlerStartTime := PerfMax(deliveryTime, node_pr);
+    var deliveryTime := TimeAdd2(pkt_ts, DeliveryTime()[delivery_idx]);
+    var handlerStartTime := TimeMax(deliveryTime, node_ts);
     var step_idx := num_steps.num_hsteps[hstep];
-    var total_time := PerfAdd2(handlerStartTime, PerfStep(hstep)[step_idx]);
+    var total_time := TimeAdd2(handlerStartTime, StepTime(hstep)[step_idx]);
     var num_steps' := num_steps.(num_hsteps := num_steps.num_hsteps[hstep := num_steps.num_hsteps[hstep] + 1], num_deliveries := num_steps.num_deliveries + 1);
     (total_time, num_steps')
   }
