ironfleet/src/Dafny/Distributed/Protocol/Lock/PerformanceProof/Definitions.i.dfy
@@ -1,161 +1,71 @@
 // Must be verified with /arith:2
 
-include "../../../Services/Lock/LockTaggedDistributedSystem.i.dfy"
+include "../../../Services/Lock/LockTimestampedDistributedSystem.i.dfy"
 
 module PerformanceProof__Definitions_i {
-import opened LockTaggedDistributedSystem_i
+import opened LockTimestampedDistributedSystem_i
 
-ghost const Gs := PerfStep(GrantStep);
-ghost const As := PerfStep(AcceptStep);
-ghost const Ds := PerfDelivery();
-ghost const G:PerfObject
-ghost const A:PerfObject
-ghost const D:PerfObject
+ghost const Gs := StepTime(GrantStep);
+ghost const As := StepTime(AcceptStep);
+ghost const Ds := DeliveryTime();
+ghost const G:Timestamp
+ghost const A:Timestamp
+ghost const D:Timestamp
 
-function StepToTimeDelta(hstep:HostStep) : PerfReport
+function StepToTimeDelta(hstep:HostStep) : Timestamp
 {
   if hstep == GrantStep then G else A
 }
 
-function TLS_NoRecvPerfUpdate(node_pr:PerfReport, hstep:HostStep) : PerfExpr
+function TLS_NoRecvPerfUpdate(node_pr:Timestamp, hstep:HostStep) : Timestamp
 {
-  var total_time := PerfAdd2(node_pr, StepToTimeDelta(hstep));
+  var total_time := TimeAdd2(node_pr, StepToTimeDelta(hstep));
   total_time
 }
 
-function TLS_RecvPerfUpdate(node_pr:PerfExpr, pkt_pr:PerfExpr, hstep:HostStep) : PerfExpr
+function TLS_RecvPerfUpdate(node_pr:Timestamp, pkt_pr:Timestamp, hstep:HostStep) : Timestamp
 {
-  var deliveryTime := PerfAdd2(pkt_pr, D);
-  var handlerStartTime := PerfMax(deliveryTime, node_pr);
-  var total_time := PerfAdd2(handlerStartTime, StepToTimeDelta(hstep));
+  var deliveryTime := TimeAdd2(pkt_pr, D);
+  var handlerStartTime := TimeMax(deliveryTime, node_pr);
+  var total_time := TimeAdd2(handlerStartTime, StepToTimeDelta(hstep));
   total_time
 }
 
-function PerfBoundLockHeld(epoch: int) : PerfExpr
+function PerfBoundLockHeld(epoch: int) : Timestamp
   requires 0 < epoch
 {
   (epoch - 1) * G + (epoch - 1) * A + (epoch - 1) * D
 }
 
-function PerfBoundLockInNetwork(epoch: int) : PerfExpr
+function PerfBoundLockInNetwork(epoch: int) : Timestamp
   requires 1 < epoch
 {
   (epoch - 1) * G + (epoch - 2) * A + (epoch - 2) * D
 }
 
-predicate PerfEq(p1:PerfObject, p2:PerfObject)
+predicate TimeEq(p1:Timestamp, p2:Timestamp)
 {
   p1 == p2
 }
 
-predicate PerfLe(p1:PerfObject, p2:PerfObject)
+predicate PerfLe(p1:Timestamp, p2:Timestamp)
 {
   p1 <= p2
 }
 
 lemma Grant_j_helper_specific(epoch:int)
   requires epoch > 0
-  ensures PerfEq(PerfBoundLockInNetwork(epoch + 1), PerfAdd2(PerfBoundLockHeld(epoch), G));
+  ensures TimeEq(PerfBoundLockInNetwork(epoch + 1), TimeAdd2(PerfBoundLockHeld(epoch), G));
 {
 }
 
 lemma Grant_j_helper()
-  ensures forall epoch :: epoch > 0 ==> PerfEq(PerfBoundLockInNetwork(epoch + 1), PerfAdd2(PerfBoundLockHeld(epoch), G));
+  ensures forall epoch :: epoch > 0 ==> TimeEq(PerfBoundLockInNetwork(epoch + 1), TimeAdd2(PerfBoundLockHeld(epoch), G));
 {
 }
 
 lemma Accept_j_helper()
-  ensures forall epoch :: epoch > 1 ==> PerfEq(PerfBoundLockHeld(epoch), TLS_RecvPerfUpdate(PerfVoid(), PerfBoundLockInNetwork(epoch), AcceptStep))
+  ensures forall epoch :: epoch > 1 ==> TimeEq(PerfBoundLockHeld(epoch), TLS_RecvPerfUpdate(TimeVoid(), PerfBoundLockInNetwork(epoch), AcceptStep))
 {
 }
-
-// lemma lemma_Accept_j_PR(pkt_pr:PerfReport, node_pr:PerfReport, node_pr':PerfReport, epoch:int, num_steps:NumSteps)
-//   requires 1 < epoch
-//   requires node_pr' == RecvPerfUpdate(node_pr, pkt_pr, AcceptStep, num_steps).0;
-//   requires pkt_pr == PerfBoundLockInNetwork(epoch)
-//   requires node_pr == PerfVoid()
-//   ensures PerfEq(node_pr', PerfBoundLockHeld(epoch))
-// {
-//   PerfProperties(); 
-// 
-//   var s : multiset<PerfExpr> := multiset{};
-//   var s2 := s[PerfStep(GrantStep) := epoch - 1];
-//   var s3 := s[PerfStep(AcceptStep) := epoch - 2];
-//   var s3' := s[PerfStep(AcceptStep) := epoch - 1];
-//   var s4 := s[PerfDelivery() := epoch - 2];
-//   var s4' := s[PerfDelivery() := epoch - 1];
-//   var sNetwork := s2 + s3 + s4;
-//   var sDelivery := s2 + s3 + s4';
-//   var sHeld := s2 + s3' + s4';
-// 
-//   assert sDelivery == sNetwork + multiset{PerfDelivery()};
-//   assert sHeld == sDelivery + multiset{PerfStep(AcceptStep)};
-// }
-
-/*
-
-lemma Test(j:int)
-  requires 1 < j
-{
-  PerfProperties();
-  quotient_axioms();
-  var p := quotient_map(PerfVoid);
-  var p' := quotient_map(PerfBoundLockHeld(j));
-  var pkt_pr := quotient_map(PerfBoundLockInNetwork(j));
-
-  var deliveryTime := PerfAdd(pkt_pr, quotient_map(PerfDelivery));
-  var handlerStartTime := PerfMax(deliveryTime, p);
-  var totalTime := PerfAdd(handlerStartTime, quotient_map(PerfStep(AcceptStep)));
-
-  assert totalTime == p';
-}
-
-lemma specific_axiom(a:multiset<PerfExpr>, b:multiset<PerfExpr>)
-  ensures PerfEq(PerfAdd(b + multiset{PerfAdd(a)}), PerfAdd(b + a))
-{
-}
-
-lemma Other(j:int, pkt_pr: PerfReport, nd_pr:PerfReport, final_pr:PerfReport)
-  requires 1 < j;
-  requires PerfEq(pkt_pr, PerfBoundLockInNetwork(j));
-  // requires PerfEq(nd_pr, PerfVoid);
-  requires nd_pr == PerfVoid;
-  ensures PerfEq(PerfAdd2(PerfMax(multiset{PerfAdd2(pkt_pr, PerfDelivery), nd_pr}), PerfStep(AcceptStep)), PerfBoundLockHeld(j));
-{
-  Test(j, pkt_pr, nd_pr, final_pr);
-}
-
-
-lemma Test(j:int, pkt_pr: PerfReport, nd_pr:PerfReport, final_pr:PerfReport)
-  requires 1 < j;
-  // requires PerfEq(pkt_pr, PerfBoundLockInNetwork(j));
-  requires pkt_pr == PerfBoundLockInNetwork(j);
-  // requires PerfEq(nd_pr, PerfVoid);
-  requires nd_pr == PerfVoid;
-  ensures PerfEq(PerfAdd2(PerfMax(multiset{PerfAdd2(pkt_pr, PerfDelivery), nd_pr}), PerfStep(AcceptStep)), PerfBoundLockHeld(j));
-
-{
-  PerfProperties();
-// 
-  // var p := PerfVoid;
-  // var p' := PerfBoundLockHeld(j);
-  // // var pkt_pr := PerfBoundLockInNetwork(j);
-// 
-  // var deliveryTime := PerfAdd2(pkt_pr, PerfDelivery);
-  // var handlerStartTime := PerfMax(multiset{deliveryTime, p});
-  // var totalTime := PerfAdd2(handlerStartTime, PerfStep(AcceptStep));
-// 
-  // assert PerfEq(totalTime, p');
-}
-
-// if |ios| > 0 && ios[0].LIoOpReceive? then
-  // var deliveryTime := PerfAdd2(ios[0].pr, PerfDeliver);
-  // var handlerStartTime := PerfMax(multiset{deliveryTime, tagged_node_state.pr});
-  // var totalTime := PerfAdd2(handlerStartTime, PerfStep(GrantStep));
-  //
-// else
-  // var totalTime := PerfAdd2(ios[0].pr, PerfStep(GrantStep));
-
-*/
-  
 }
